Simu/Cor.v
@@ -45,6 +45,8 @@ Section PRESERVATION.
 
   Hypothesis TRANSL: translate prog main_node = Errors.OK tprog.
   Hypothesis main_node_exists: find_class main_node prog <> None.
+  Hypothesis WD: WelldefClasses prog.
+  
   (* Hypothesis UNIQUE: unique_classes prog. *)
   
   (* Hypothesis WF: well_formed prog. *)
@@ -125,12 +127,14 @@ Section PRESERVATION.
       (* Nelist.length ys = Nelist.length rvs -> *)
       (* Nelist.Forall (fun y => In y (class_vars c)) ys -> *)
       (* y <> self_id -> *)
-      (* In {| obj_inst := o; obj_class := clsid |} c.(c_objs) -> *)
+      length ys = length f.(m_out) ->
+      In (o, clsid) c.(c_objs) ->
+      In (o, clsid, fid) (get_instance_methods m.(m_body)) ->
       (* find_class clsid prog = Some (c', prog') -> *)
       Forall (well_formed_exp c m) es ->
       (* Nelist.Forall2 (exp_eval S) es vs -> *)
       (* Nelist.Forall2 (fun e v => valid_val v (typeof e)) es vs -> *)
-      (* Nelist.Forall2 (fun e x => typeof e = snd x) es c'.(c_input) -> *)
+      Forall2 (fun e x => typeof e = snd x) es f.(m_in) ->
       (* ty = snd c'.(c_output) -> *)
       (* find_inst S o me -> *)
       (* well_formed_stmt c' (me, adds (Nelist.map_fst c'.(c_input)) vs v_empty) m.(m_body) -> *)
@@ -164,8 +168,10 @@ Section PRESERVATION.
         ** sepall (fun ocg =>
                      let '(o, cid, g) := ocg in
                      match gcenv ! (prefix g cid), e!o with 
-                     | Some gco, Some (oblk, _) =>
-                       blockrep gcenv v_empty (co_members gco) oblk
+                     | Some gco, Some (oblk, t) =>
+                       if type_eq t (type_of_inst (prefix g cid)) then
+                         blockrep gcenv v_empty (co_members gco) oblk
+                       else sepfalse
                      | _, _ => sepfalse
                      end) (get_instance_methods f.(m_body))
         ** pure (Forall (fun (xty: ident * typ) =>
@@ -184,6 +190,8 @@ Section PRESERVATION.
       (0 <= Int.unsigned sofs)%Z ->
       match_states c f S (e, le, m).
 
+  Hint Constructors match_states.
+  
   Remark invariant_blockrep:
     forall c f me ve e le m sb sofs outb outco,
       sep_invariant c f (me, ve) e le m sb sofs outb outco ->
@@ -753,28 +761,326 @@ Section PRESERVATION.
         apply Notin.
         eapply In_InMembers; eauto.
   Qed.
+
+  (* Remark alloc_exists: *) 
+  (*   forall vars e m, *) 
+  (*     exists e' m', *) 
+  (*       Clight.alloc_variables tge e m vars e' m'. *) 
+  (* Proof. *) 
+  (*   induction vars as [|(x, ty)]. *) 
+  (*   - do 3 econstructor. *) 
+  (*   - intros. *) 
+  (*     destruct (Memory.Mem.alloc m 0 (Ctypes.sizeof (Clight.genv_cenv tge) ty)) eqn: Eq. *) 
+  (*     specialize (IHvars (Maps.PTree.set x (b, ty) e) m0). *) 
+  (*     destruct* IHvars as (? & ? & ?). *) 
+  (*     do 3 econstructor; eauto. *) 
+  (* Qed. *) 
+ 
+  (* Remark assign_loc_exists: *) 
+  (*   forall v ty m loc, *) 
+  (*     Ctypes.access_mode ty = Ctypes.By_value (chunk_of_type ty) -> *) 
+  (*     Memory.Mem.valid_access m (chunk_of_type ty) loc 0 Memtype.Writable -> *) 
+  (*     exists m', *) 
+  (*       Clight.assign_loc tge.(Clight.genv_cenv) ty m loc Int.zero v m'. *) 
+  (* Proof. *) 
+  (*   introv ? Hvalid. *) 
+  (*   forwards (? & ?): Memory.Mem.valid_access_store Hvalid. *) 
+  (*   do 2 econstructor; eauto. *) 
+  (* Qed. *) 
+   
+  (* Remark bind_parameters_exists: *) 
+  (*   forall xs vs e m, *) 
+  (*     length xs = length vs -> *) 
+  (*     Forall (fun x => exists loc, *) 
+  (*                 Maps.PTree.get (fst x) e = Some (loc, snd x) *) 
+  (*                 /\ Memory.Mem.valid_access m (chunk_of_type (snd x)) loc 0 Memtype.Writable *) 
+  (*                 /\ Ctypes.access_mode (snd x) = Ctypes.By_value (chunk_of_type (snd x))) xs -> *) 
+  (*     exists m', *) 
+  (*       Clight.bind_parameters tge e m xs vs m'. *) 
+  (* Proof. *) 
+  (*   induction xs as [|(x, ty)]; destruct vs; introv Hlengths Hparams; try discriminate. *) 
+  (*   - do 2 econstructor. *) 
+  (*   - inverts Hparams as (? & ? & Hvalid & Haccess) Hparams.   *) 
+  (*     forwards (m' & Hassign): (assign_loc_exists v) Haccess Hvalid. *) 
+  (*     edestruct IHxs with (m:=m') (e:=e); eauto. *) 
+  (*     + inversion_clear Hassign as [|? ? ? ? Haccess']. *) 
+  (*       *{ clear IHxs Hlengths. induction xs. *) 
+  (*          - constructor. *) 
+  (*          - inverts Hparams as (loc & ?). *) 
+  (*            constructor. *) 
+  (*            + exists loc; splits*. *) 
+  (*              apply* Memory.Mem.store_valid_access_1. *) 
+  (*            + apply* IHxs. *) 
+  (*        } *) 
+  (*       * rewrite Haccess' in Haccess; discriminate. *) 
+  (*     + do 2 econstructor; eauto.  *) 
+  (* Qed. *) 
+ 
+  (* Remark alloc_variables_implies: *) 
+  (*   forall vars e m e' m',  *) 
+  (*     Clight.alloc_variables tge e m vars e' m' -> *) 
+  (*     Forall (fun x => Ctypes.access_mode (snd x) = Ctypes.By_value (chunk_of_type (snd x))) vars -> *) 
+  (*     Forall (fun x => exists loc, *) 
+  (*                 Maps.PTree.get (fst x) e' = Some (loc, snd x) *) 
+  (*                 /\ Memory.Mem.valid_access m' (chunk_of_type (snd x)) loc 0 Memtype.Writable *) 
+  (*                 /\ Ctypes.access_mode (snd x) = Ctypes.By_value (chunk_of_type (snd x))) vars. *) 
+  (* Proof. *) 
+  (*   induction vars. *) 
+  (*   - constructor. *) 
+  (*   - introv Halloc Hforall. *) 
+  (*     inverts Halloc. *) 
+  (*     constructor. *) 
+  (*     + exists b1; splits*. *) 
+  (*       * admit. *) 
+  (*       *{ assert (Memory.Mem.valid_access m1 (chunk_of_type (snd (id, ty))) b1 0 Memtype.Writable). *) 
+  (*          - eapply Memory.Mem.valid_access_freeable_any. *) 
+  (*            apply* Memory.Mem.valid_access_alloc_same. *) 
+  (*            + omega. *) 
+  (*            + simpl. admit. *) 
+  (*            + eapply BinInt.Z.divide_0_r. *) 
+  (*          - admit. *) 
+  (*        } *) 
+  (*       * inverts* Hforall. *) 
+  (*     + apply* IHvars. *) 
+  (*       inverts* Hforall. *) 
+  (* Qed. *) 
+ 
+  (* Remark forall_app: *) 
+  (*   forall A (P: A -> Prop) l1 l2, *) 
+  (*     Forall P (l1 ++ l2) -> Forall P l1 /\ Forall P l2. *) 
+  (* Proof. *) 
+  (*   introv HForall; split; rewrite Forall_forall in *; introv Hin; *) 
+  (*   apply HForall; apply in_or_app; [left | right]; auto. *) 
+  (* Qed. *) 
+ 
+  (* Lemma compat_funcall_pres: *) 
+  (*   forall m f vargs, *) 
+  (*     Datatypes.length (Clight.fn_params f) = Datatypes.length vargs -> *) 
+  (*     Forall (fun x => Ctypes.access_mode (snd x) = Ctypes.By_value (chunk_of_type (snd x))) (f.(Clight.fn_params) ++ f.(Clight.fn_vars)) -> *) 
+  (*     exists m1 e_fun m2, *) 
+  (*       Clight.alloc_variables tge Clight.empty_env m (f.(Clight.fn_params) ++ f.(Clight.fn_vars)) e_fun m1  *) 
+  (*       /\ Clight.bind_parameters tge e_fun m1 f.(Clight.fn_params) vargs m2. *) 
+  (* Proof. *) 
+  (*   introv Hlengths Haccesses. *) 
+  (*   forwards (e_fun & m1 & Halloc): *) 
+  (*     (alloc_exists (f.(Clight.fn_params) ++ f.(Clight.fn_vars)) Clight.empty_env m). *) 
+  (*   exists m1 e_fun. *) 
+  (*   forwards* Hforall': alloc_variables_implies Halloc Haccesses. *) 
+  (*   forwards (Hforall & H'): forall_app Hforall'; clear Hforall' H'. *) 
+  (*   forwards* (m2 & ?): bind_parameters_exists Hlengths Hforall. *) 
+  (* Qed. *)
   
   (* Hint Constructors Clight.eval_lvalue Clight.eval_expr well_formed_stmt. *)
   Hint Resolve expr_eval_simu Clight.assign_loc_value exp_eval_valid sem_cast_same.
 
-  (* Hypothesis STEPS: *)
-  (*   forall c (e: Clight.env), *)
-  (*     In c prog -> *)
-  (*     exists loc_f f, *)
-  (*       Globalenvs.Genv.find_symbol tge.(Clight.genv_genv) (step_id c.(c_name)) = Some loc_f *)
-  (*       /\ Maps.PTree.get (step_id c.(c_name)) e = None *)
-  (*       /\ Globalenvs.Genv.find_funct_ptr tge.(Clight.genv_genv) loc_f = Some (Ctypes.Internal f) *)
-  (*       /\ Clight.type_of_fundef (Ctypes.Internal f) = *)
-  (*         Ctypes.Tfunction (Ctypes.Tcons (type_of_inst_p c.(c_name)) *)
-  (*                                        (list_type_to_typelist (map snd (nelist2list c.(c_input) ++ nelist2list c.(c_output))))) *)
-  (*                                        Ctypes.Tvoid AST.cc_default *)
-  (*       /\ Coqlib.list_norepet (Clight.var_names (Clight.fn_params f) ++ Clight.var_names (Clight.fn_vars f)) *)
-  (*       /\ Clight.fn_body f = snd (translate_stmt c.(c_name) c.(c_step)) *)
-  (*       /\ length f.(Clight.fn_params) = 1 + Nelist.length c.(c_input)   *)
-  (*       /\ Forall (fun x => Ctypes.access_mode (snd x) = Ctypes.By_value (chunk_of_type (snd x))) *)
-  (*                (f.(Clight.fn_params) ++ f.(Clight.fn_vars)). *)
+  Lemma methods_corres:
+    forall c clsnm prog' mid m (e: Clight.env),
+      find_class clsnm prog = Some (c, prog') ->
+      find_method mid c.(c_methods) = Some m ->
+      exists loc_f f,
+        Genv.find_symbol tge mid = Some loc_f
+        /\ e ! mid = None
+        /\ Genv.find_funct_ptr tge loc_f = Some (Internal f)
+        /\ type_of_function f =
+          Tfunction
+            (Ctypes.Tcons (type_of_inst_p c.(c_name))
+                          (Ctypes.Tcons (type_of_inst_p (prefix m.(m_name) c.(c_name)))
+                                        (list_type_to_typelist (map snd m.(m_in)))))
+            Tvoid AST.cc_default
+  (* /\ type_of_fundef (Internal f) = *)
+        (*   Tfunction (Ctypes.Tcons (type_of_inst_p c.(c_name)) *)
+        (*                           (Ctypes.Tcons (type_of_inst_p (prefix m.(m_name) c.(c_name))) *)
+        (*                                         (list_type_to_typelist (map snd m.(m_in))))) *)
+        (*             Tvoid AST.cc_default *)
+        (* /\ Coqlib.list_norepet (Clight.var_names (Clight.fn_params f) ++ Clight.var_names (Clight.fn_vars f)) *)
+        (* /\ Clight.fn_body f = snd (translate_stmt c.(c_name) c.(c_step)) *)
+        (* /\ length f.(Clight.fn_params) = 1 + Nelist.length c.(c_input) *)
+        (* /\ Forall (fun x => Ctypes.access_mode (snd x) = Ctypes.By_value (chunk_of_type (snd x))) *)
+        (*          (f.(Clight.fn_params) ++ f.(Clight.fn_vars)) *).
+  Admitted.
   
-  Check stmt_eval_call_ind.
+  Lemma eval_self_inst:
+    forall clsnm prog' c f S e le m o c' sb sofs outb outco,
+      find_class clsnm prog = Some (c, prog') ->
+      In f c.(c_methods) ->
+      le ! self_id = Some (Vptr sb sofs) ->
+      sep_invariant c f S e le m sb sofs outb outco ->
+      In (o, c') (c_objs c) ->
+      exists d,
+        eval_expr tge e le m (ptr_obj c.(c_name) c' o) (Vptr sb (Int.add sofs (Int.repr d))).
+  Proof.
+    introv Find ? ? Hrep Hin.
+    destruct S.
+    forwards ?: find_class_name Find; subst.
+    eapply invariant_staterep in Hrep; eauto.
+    forwards* (? & Hco & ? & Eq & ? & ?): make_members_co; instantiate (1:=tprog) in Hco.
+    forwards* (d & Hoffset): staterep_inst_offset. 
+    exists d.
+    apply eval_Eaddrof.
+    apply* eval_Efield_struct.
+    - apply* eval_Elvalue.
+      apply* deref_loc_copy. 
+    - simpl; unfold type_of_inst; eauto.
+    - rewrite* Eq. 
+  Qed.
+
+  Lemma evall_out_struct:
+    forall clsnm prog' c f f' S e le m o ty c' sb sofs outb outco,
+      find_class clsnm prog = Some (c, prog') ->
+      In f c.(c_methods) ->
+      le ! self_id = Some (Vptr sb sofs) ->
+      sep_invariant c f S e le m sb sofs outb outco ->
+      In (o, c', f') (get_instance_methods f.(m_body)) ->
+      ty = type_of_inst (prefix f' c') ->
+      exists b,
+        eval_lvalue tge e le m (Evar o ty) b Int.zero.
+  Proof.
+    introv Find ? ? Hrep Hin ?; subst.
+    destruct S.
+    forwards ?: find_class_name Find; subst.
+    apply sep_pick3 in Hrep.
+    apply sepall_in in Hin; destruct Hin as [ws [xs [Hsplit Hin]]].
+    rewrite Hin in Hrep. clear Hsplit Hin.
+    apply sep_proj1 in Hrep.
+    clear ws xs.
+    destruct gcenv ! (prefix f' c'); [|contradict Hrep].
+    destruct e ! o eqn: E; [|contradict Hrep].
+    destruct p as (oblk, t).
+    destruct (type_eq t (type_of_inst (prefix f' c'))); [|contradict Hrep].
+    subst.
+    exists oblk.
+    apply* eval_Evar_local.
+  Qed.  
+
+  Remark type_pres':
+    forall f c caller es,
+      Forall2 (fun e x => typeof e = snd x) es f.(m_in) ->
+      map snd f.(m_in) = map Clight.typeof (map (translate_exp c caller) es).
+  Proof.
+    intro f.
+    induction (m_in f); introv Heq; inversion_clear Heq as [|? ? ? ? Ht]; simpl; auto.
+    f_equal.
+    - rewrite <-Ht.
+      rewrite* type_pres.
+    - apply* IHl.
+  Qed.
+
+  (* Lemma exec_assign: *)
+  (*   forall e1 le1 m1 clsnm prog' c S f x e v sb sofs outb outco, *)
+  (*     find_class clsnm prog = Some (c, prog') -> *)
+  (*     In f c.(c_methods) -> *)
+  (*     well_formed_exp c f e -> *)
+  (*     In (x, typeof e) (meth_vars f) -> *)
+  (*     le1 ! self_id = Some (Vptr sb sofs) -> *)
+  (*     (0 <= Int.unsigned sofs)%Z -> *)
+  (*     le1 ! out_id = Some (Vptr outb Int.zero) -> *)
+  (*     gcenv ! (prefix f.(m_name) c.(c_name)) = Some outco -> *)
+  (*     sep_invariant c f S e1 le1 m1 sb sofs outb outco -> *)
+  (*     exp_eval S e v -> *)
+  (*     exists le2 m2 T, *)
+  (*       exec_stmt tge (function_entry2 tge) e1 le1 m1 *)
+  (*                 (translate_stmt prog c f (Assign x e)) T le2 m2 Out_normal *)
+  (*       /\ match_states c f (update_var S x v) (e1, le2, m2). *)
+  (* Proof. *)
+  (*   introv ? ? ? Hvars; intros. *)
+  (*   simpl. *)
+  (*   simpl; unfold assign. *)
+  (*   destruct (existsb (fun out => ident_eqb (fst out) x) f.(m_out)) eqn: E. *)
+    
+  (*   (* out->x = e *) *)
+  (*   - (* get the 'out' variable left value evaluation *) *)
+  (*     edestruct evall_out_field; eauto. *)
+      
+  (*     (* get the updated memory *) *)
+  (*     edestruct match_states_assign_out as (m2 & ?); jauto. *)
+        
+  (*     exists le1 m2 E0; split*. *)
+  (*     apply* ClightBigstep.exec_Sassign. *)
+  (*     + rewrite* type_pres; apply* sem_cast_same; apply* exp_eval_valid. *)
+  (*     + apply* assign_loc_value. *)
+  (*       * simpl; apply* exp_eval_access. *)
+  (*       * rewrite* Int.add_zero_l. *)
+          
+  (*   (* x = e *) *)
+  (*   - exists (PTree.set x v le1) m1 E0; split. *)
+  (*     + apply* ClightBigstep.exec_Sset. *)
+  (*     + pose proof (m_out_id f); pose proof (m_self_id f). *)
+  (*       apply* match_states_assign_tempvar; *)
+  (*         apply In_InMembers in Hvars; eapply InMembers_neq; eauto. *)
+  (* Qed. *)
+  
+  Lemma exec_funcall_assign:
+    forall callee caller ys e1 le1 m1 c prog' c' prog'' o f clsid S sb sofs outb outco instco,  
+      find_class c.(c_name) prog = Some (c, prog') ->
+      In caller c.(c_methods) ->
+      find_class clsid prog = Some (c', prog'') ->
+      find_method f c'.(c_methods) = Some callee ->
+      gcenv ! (prefix f clsid) = Some instco ->
+      In (o, clsid, f) (get_instance_methods caller.(m_body)) ->
+      length ys = length callee.(m_out) ->
+      Forall (fun y => In y (meth_vars caller)) ys ->
+      le1 ! out_id = Some (Vptr outb Int.zero) ->
+      le1 ! self_id = Some (Vptr sb sofs) ->
+      sep_invariant c caller S e1 le1 m1 sb sofs outb outco ->
+      gcenv ! (prefix caller.(m_name) c.(c_name)) = Some outco ->
+      exists le2 m2 T,
+        exec_stmt tge (function_entry2 tge) e1 le1 m1
+                  (funcall_assign ys c.(c_name) caller o (type_of_inst (prefix f clsid)) callee)
+                  T le2 m2 Out_normal.
+  Proof.
+    unfold funcall_assign.
+    introv Findc ? ? ? Hinstco ? Length Hforall; intros.
+    revert le1 m1 H3 H4 H5 ys Hforall Length.
+    induction (m_out callee); introv Hforall Length;    
+    destruct ys; simpl in *; try discriminate.
+    - exists le1 m1 E0; apply exec_Sskip.
+    - destruct p as (y, ty); destruct a as (y', ty').
+      inverts Length.
+      inverts Hforall.
+      (* forwards Eq: find_class_name Findc. *)
+      (* forwards Eq': find_method_name Findmeth. *)
+      (* edestruct IHl as (? & ? & ? & ?); eauto. *)
+      (* clear IHl. *)
+      (* unfold assign. *)
+      (* destruct (existsb (fun out => ident_eqb (fst out) y) caller.(m_out)) eqn: E. *)
+
+      (* (* out->y = o.y' *) *)
+      (* + (* get the 'out' variable left value evaluation *) *)
+      (*   forwards* (? & ? & ?): evall_out_field Findc. *)
+
+      (*   (* get the o struct left value evaluation *) *)
+      (*   forwards* (? & ?): evall_out_struct Findc. *)
+
+      (*   do 3 econstructor. *)
+      (*   apply* exec_Sseq_1. *)
+      (*   apply* ClightBigstep.exec_Sassign. *)
+      (*   *{ apply* eval_Elvalue. *)
+      (*      - eapply eval_Efield_struct. *)
+      (*        + apply* eval_Elvalue. *)
+      (*          apply* deref_loc_copy. *)
+      (*        + unfold type_of_inst; simpl; eauto.   *)
+      (*        + eauto. *)
+      (*        + skip. *)
+      (*      - apply* deref_loc_value. *)
+      (*        + simpl. skip. *)
+      (*        + skip. *)
+      (*    } *)
+      (*   * simpl; apply* sem_cast_same. skip. *)
+      (*   *{ apply* assign_loc_value. *)
+      (*      - simpl. skip. *)
+      (*      - rewrite Int.add_zero_l. *)
+      (*        skip. *)
+      (*    } *)
+
+      (* (* x = e *) *)
+      (* + do 3 econstructor. *)
+      (*   apply* exec_Sseq_1. *)
+      (*   apply* ClightBigstep.exec_Sset. *)
+      (*   * pose proof (m_out_id f); pose proof (m_self_id f). *)
+      (*     apply* match_states_assign_tempvar;  *)
+      (*       apply In_InMembers in Hvars; eapply InMembers_neq; eauto. *)
+Admitted.
+  
   Theorem correctness:
     (forall p S1 s S2,
         stmt_eval p S1 s S2 ->
@@ -793,23 +1099,26 @@ Section PRESERVATION.
     (forall p me1 clsid fid vs me2 rvs,
         stmt_call_eval p me1 clsid fid vs me2 rvs ->
         sub_prog p prog ->
-        forall c caller S e1 le1 m1 o self out f ptr_f,
-          match_states c caller S (e1, le1, m1) ->
+        forall c caller S e1 le1 m1 o f ptr_f sb o_ofs outb oty
+          (MS: match_states c caller S (e1, le1, m1)),
           Globalenvs.Genv.find_symbol tge fid = Some ptr_f ->
           Globalenvs.Genv.find_funct_ptr tge ptr_f = Some (Ctypes.Internal f) ->
           find_inst S o me1 ->
+          oty = type_of_inst (prefix fid clsid) ->
+          eval_expr tge e1 le1 m1 (ptr_obj c.(c_name) clsid o) (Vptr sb o_ofs) ->
+          eval_expr tge e1 le1 m1 (Eaddrof (Evar o oty) (pointer_of oty)) (Vptr outb Int.zero) ->
           exists m2 T,
             eval_funcall tge (function_entry2 tge) m1 (Internal f)
-                         (self :: out :: vs) T m2 Vundef
+                         ((Vptr sb o_ofs) :: (Vptr outb Int.zero) :: vs) T m2 Vundef
             /\ match_states c caller (update_inst S o me2) (e1, le1, m2)).
   Proof.
     clear TRANSL main_node_exists.
     apply stmt_eval_call_ind;
       [| |introv ? ? ? ? Hifte|introv ? HS1 ? HS2|introv ? Evs ? Hrec_eval|
-       |];
+       |introv Find ? ? Hrec_exec];
       intros;
-      try inversion_clear WF as [? ? Hvars|? ? Hin| | |? ? ? ? ? ? ? ? ? Find' Findmeth|];
-      try (pose proof MS as MS'; inverts MS' as Hself Hout Houtco Hrep).
+      try inversion_clear WF as [? ? Hvars|? ? Hin| | |? ? ? ? ? ? ? ? ? ? ? ? ? Find' Findmeth|];
+      pose proof MS as MS'; inverts MS' as Hself Hout Houtco Hrep.
     
     (* Assign x e : "x = e" *)
     - simpl; unfold assign.
@@ -868,25 +1177,26 @@ Section PRESERVATION.
     (* Step_ap y ty clsid o [e1; ... ;en] : "y = clsid_step(&(self->o), e1, ..., en)" *)
     - (* get the Clight corresponding function *)
       forwards* Hin': find_class_In Find'.
-      (* pose proof Hstep as Hstep'. *)
-      (* edestruct Hstep' as (loc_f & f & ? & ? & ? & Htype_fun & ? & ? & Hlengths & ?); eauto. *)
-      (* rewrite <-type_pres' with (c:=c) (es:=es) (ys:=ys) in Htype_fun; auto. *)
-      forwards Eq: find_class_name Find'.
-      (* rewrite Eq in *; clear Eq. *)
-      
-      (* get the Clight corresponding field *)
-      (* pose proof Hself as Hself'. *)
-      (* destruct* Hself' as (? & ? & ? & ? & ? & ? & ? & ? & Hobj). *)
-      (* specializes Hobj Hin; destruct Hobj. *)
+      edestruct methods_corres with (e:=e1) as (ptr_f & cf & ? & ? & ? & Htypefun); eauto.
 
-      (* get outs values *)
-      (* edestruct exprlist_make_out_arg with (le:=le1) (c:=c) as (outs); eauto. *)
+      forwards Eq: find_class_name Find'.
+      forwards Eq': find_method_name Findmeth.
+      rewrite Eq, Eq' in *.
+
+      (* the *self parameter *)
+      edestruct eval_self_inst with (1:=Find); eauto.
+      
+      (* the *out parameter *)
+      edestruct evall_out_struct with (1:=Find) (o:=o) (c':=clsid) (f':=f); eauto.        
       
       (* recursive funcall evaluation *)
       edestruct Hrec_eval with (c:=c) (e1:=e1) (m1:=m1) (le1:=le1) as (m2 & T & ? & ?); eauto.
-      skip.                     (* f ∈ tge *)
-      skip.                     (* f points to the function *)
-      exists le1 m2; econstructor; split.
+
+      (* output assignments *)
+      edestruct exec_funcall_assign with (ys:=ys) as (? & ? & ? & ?) ; eauto.
+      skip. admit. admit.
+      (* TODO write a lemma which gives the right state *)
+      do 3 econstructor; split.
       + simpl.
         unfold binded_funcall.
         rewrite Find', Findmeth.
@@ -895,46 +1205,31 @@ Section PRESERVATION.
            - reflexivity.
            - simpl.
              eapply eval_Elvalue.
-             + apply eval_Evar_global.
-               * skip.          (* f ∉ e₁ *)
-               * skip.          (* f ∈ tge *)
+             + apply* eval_Evar_global.
              + apply* deref_loc_reference.               
            - apply find_method_In in Findmeth.
-             econstructor.
-             + eapply Clight.eval_Eaddrof. 
-               skip.            (* left-evaluation of self->o *)
-             + eapply sem_cast_same. 
-               unfold valid_val; splits*.
-               * discriminate. 
-               * simpl; trivial.
-             + econstructor.
-               * eapply Clight.eval_Eaddrof. 
-                 skip.          (* left-evaluation of the out structure o *)
-               *{ eapply sem_cast_same. 
-                  unfold valid_val; splits*.
-                  - discriminate. 
-                  - simpl; trivial.
-                }
-               * applys* exprs_eval_simu Find.
-           - skip.              (* f points to the function *)
-           - skip.              (* type of the function *)
+             do 2 (econstructor; eauto).
+             applys* exprs_eval_simu Find.
+           - unfold Genv.find_funct.
+             destruct* (Int.eq_dec Int.zero Int.zero) as [|Neq].
+             exfalso; apply* Neq.
+           - simpl; rewrite Htypefun; repeat f_equal.
+             apply* type_pres'.
          }
-        * simpl.
-          skip.                 (* ouput assignments *)
+        * 
       + skip.
       
     (* Skip : "skip" *)
-    - do 3 econstructor; split*.
+    - exists le1 m1 E0; split*.
       eapply exec_Sskip.
 
     (* funcall *)
-    - admit.
-      (* forwards* Hfind'': find_class_sub_same Hfind UNIQUE. *)
+    - forwards* Find'': find_class_sub_same.
       (* rewrite Hfind' in Hfind''; inverts Hfind''. *)
       (* destruct Hstep with (c:=cls) *)
       (*   as (loc_f' & f' & Hget_loc_f' & Hget_f' & Htype_fun & Hvars_nil & ? & ? & Htr & ?); *)
       (*   destruct_conjs; eauto. *)
-      (* forwards Eq: find_class_name Hfind. *)
+      forwards Eq: find_class_name Find.
       (* rewrite Eq in Hget_loc_f'; clear Eq. *)
       (* rewrite Hget_loc_f' in Hget_loc_f; inverts Hget_loc_f. *)
       (* rewrite Hget_f' in Hget_f; inverts Hget_f. *)
@@ -943,33 +1238,33 @@ Section PRESERVATION.
       (*   by (rewrite Hlengths; simpl; f_equal; rewrite Nelist.nelist2list_length; auto). *)
 
       (* forwards* (le_fun & ? & ?): (compat_funcall_pres cls m). *)
-      (* forwards* Hsub: find_class_sub. *)
+      forwards* Hsub: find_class_sub.
       (* subst env. *)
-      (* edestruct Hrec_exec with (le1:=le_fun) as (? & ? & ? & ? & MS); eauto. *)
-      (* destruct_conjs. *)
+      edestruct Hrec_exec with (le1:=le_fun) as (? & ? & ? & ? & MS); eauto.
+      destruct_conjs.
         
-      (* do 2 econstructor; split. *)
-      (* apply* eval_funcall_internal. *)
-      (* + constructor*; rewrite Hvars_nil; simpl; constructor. *)
-      (* + rewrite* Htr. *)
-      (*   apply* exec_Sseq_1. *)
-      (*   apply* exec_Sreturn_some. *)
-      (*   apply* Clight.eval_Etempvar. *)
-      (*   inverts MS as Hvars'. *)
-      (*   apply* Hvars'; rewrite <-surjective_pairing; eapply in_eq. *)
-      (* + simpl; split*. *)
-      (*   inverts Htype_fun. *)
-      (*   apply* sem_cast_same. *)
-      (* + simpl; eauto.        *)
-      (* + constructor*. *)
-      (*   unfold compat_self. *)
-      (*   intro Hin. *)
-      (*   pose proof Hself as Hself'. *)
-      (*   destruct* Hself' as (? & loc_struct' & ofs' & Hget_self' & Hget_co' & Hmem & Hobj). *)
-      (*   do 3 econstructor; splits*. *)
-      (*   intros x' t' Hin'.  *)
-      (*   specializes Hmem Hin'; destruct Hmem. *)
-      (*   econstructor; splits*. *)
-      (*   * admit. *)
-      (*   * admit. *)
+      do 2 econstructor; split.
+      apply* eval_funcall_internal.
+      + constructor*; rewrite Hvars_nil; simpl; constructor.
+      + rewrite* Htr.
+        apply* exec_Sseq_1.
+        apply* exec_Sreturn_some.
+        apply* Clight.eval_Etempvar.
+        inverts MS as Hvars'.
+        apply* Hvars'; rewrite <-surjective_pairing; eapply in_eq.
+      + simpl; split*.
+        inverts Htype_fun.
+        apply* sem_cast_same.
+      + simpl; eauto.
+      + constructor*.
+        unfold compat_self.
+        intro Hin.
+        pose proof Hself as Hself'.
+        destruct* Hself' as (? & loc_struct' & ofs' & Hget_self' & Hget_co' & Hmem & Hobj).
+        do 3 econstructor; splits*.
+        intros x' t' Hin'.
+        specializes Hmem Hin'; destruct Hmem.
+        econstructor; splits*.
+        * admit.
+        * admit.
   Qed.
